tools/gomad4/conformance/replay_test.go
@@ -4,8 +4,8 @@ import (
 	"errors"
 	"testing"
 
-	"go.temporal.io/server/tools/gomadv4/trace"
-	"go.temporal.io/server/tools/gomadv4/virtualtime"
+	"go.temporal.io/server/tools/gomad4/trace"
+	"go.temporal.io/server/tools/gomad4/virtualtime"
 )
 
 func TestReplayAcceptsBehaviorAndRejectionCases(t *testing.T) {
