tools/gomad4/internal/formalbridge/generate_test.go
@@ -3,8 +3,8 @@ package formalbridge
 import (
 	"testing"
 
-	"go.temporal.io/server/tools/gomadv4/conformance"
-	"go.temporal.io/server/tools/gomadv4/trace"
+	"go.temporal.io/server/tools/gomad4/conformance"
+	"go.temporal.io/server/tools/gomad4/trace"
 )
 
 func TestGenerateCoversEveryVirtualTimeActionAndRejection(t *testing.T) {
