tools/gomad4/regenerate/verify_test.go
@@ -6,8 +6,8 @@ import (
 	"path/filepath"
 	"testing"
 
-	"go.temporal.io/server/tools/gomadv4/trace"
-	"go.temporal.io/server/tools/gomadv4/virtualtime"
+	"go.temporal.io/server/tools/gomad4/trace"
+	"go.temporal.io/server/tools/gomad4/virtualtime"
 )
 
 func TestVerifyRegeneratesTwiceAndComparesCompleteOutput(t *testing.T) {
