tools/gomad4/trace/corpus.go
@@ -1,0 +1,58 @@
+package trace
+
+import (
+	sharedtrace "go.temporal.io/server/tools/common/formal/trace"
+	"go.temporal.io/server/tools/gomad4/virtualtime"
+)
+
+const CorpusSchema = "gomadv4.virtual-time-corpus/v1"
+
+type GenerationContract = sharedtrace.GenerationContract
+
+type Corpus = sharedtrace.Corpus[
+	virtualtime.StateSnapshot,
+	virtualtime.Action,
+	virtualtime.ObservableDelta,
+	virtualtime.RejectionCode,
+]
+
+type BehaviorTrace = sharedtrace.BehaviorTrace[
+	virtualtime.StateSnapshot,
+	virtualtime.Action,
+	virtualtime.ObservableDelta,
+]
+
+type StepRecord = sharedtrace.StepRecord[
+	virtualtime.Action,
+	virtualtime.ObservableDelta,
+]
+
+type RejectionCase = sharedtrace.RejectionCase[
+	virtualtime.StateSnapshot,
+	virtualtime.Action,
+	virtualtime.RejectionCode,
+]
+
+var codec = sharedtrace.Codec[
+	virtualtime.StateSnapshot,
+	virtualtime.Action,
+	virtualtime.ObservableDelta,
+	virtualtime.RejectionCode,
+]{
+	Subject:              "virtual time",
+	CorpusSchema:         CorpusSchema,
+	SemanticDigestDomain: "gomadv4.virtual-time-corpus-semantic/v1",
+	CorpusDigestDomain:   "gomadv4.virtual-time-corpus/v1",
+}
+
+func Finalize(corpus *Corpus) error {
+	return codec.Finalize(corpus)
+}
+
+func Encode(corpus Corpus) ([]byte, error) {
+	return codec.Encode(corpus)
+}
+
+func Decode(data []byte) (Corpus, error) {
+	return codec.Decode(data)
+}
