tools/common/formal/go.mod
@@ -1,0 +1,3 @@
+module go.temporal.io/server/tools/common/formal
+
+go 1.27.0
