tools/gomad4/go.mod
@@ -1,0 +1,7 @@
+module go.temporal.io/server/tools/gomad4
+
+go 1.27.0
+
+require go.temporal.io/server/tools/common/formal v0.0.0
+
+replace go.temporal.io/server/tools/common/formal => ../common/formal
